theories/goedel/rosser.v
@@ -31,7 +31,7 @@ Hypothesis extendsNN : Included _ NN T.
 Variable repT : Formula.
 Variable v0 : nat.
 Hypothesis
-  freeVarRepT : forall v : nat, In v (freeVarFormula LNN repT) -> v = v0.
+  freeVarRepT : forall v : nat, In v (freeVarF LNN repT) -> v = v0.
 Hypothesis
   expressT1 :
     forall f : Formula,
@@ -180,7 +180,7 @@ Qed.
 Theorem Rosser'sIncompleteness :
  (forall x : Formula, mem _ T x \/ ~ mem _ T x) ->
  exists f : Formula,
-   (forall v : nat, ~ In v (freeVarFormula LNN f)) /\
+   (forall v : nat, ~ In v (freeVarF LNN f)) /\
    (SysPrf T f \/ SysPrf T (notH f) -> Inconsistent LNN T).
 Proof.
   intros decide.
@@ -194,7 +194,7 @@ Proof.
   destruct (FixPointLNN A 0) as [x [H0 H1]].
   exists x; split.
   -  intros v H; induction (H1 v) as [H2 H3]. 
-     assert (H4: In v (List.remove eq_nat_dec 0 (freeVarFormula LNN A)))
+     assert (H4: In v (List.remove eq_nat_dec 0 (freeVarF LNN A)))
      by apply H2, H.
      unfold A in H4; SimplFreeVar.
      + assert (H4: v <= 1).
@@ -369,7 +369,7 @@ Proof.
                              (substF LNN codeSysPrfNot 0
                                 (natToTerm (codeFormula x))) 1 (natToTerm n))) rec)
                   (codePrf x0 x x1)).
-           assert (H4: forall x : nat, ~ In x (freeVarFormula LNN E)).
+           assert (H4: forall x : nat, ~ In x (freeVarF LNN E)).
            { unfold E; clear H3 E; induction (codePrf x0 x x1) as [ | n IHn].
             - simpl; auto.
             - intros x2; unfold nat_rec, nat_rect; intro H3. 
@@ -544,7 +544,7 @@ Proof.
                                    (substF LNN codeSysPrf 0 
                                       (natToTerm (codeFormula x)))
                                    1 (natToTerm n))) rec) (S (codePrf _ _ x1))). 
-                 assert (H4: forall x : nat, ~ In x (freeVarFormula LNN E)).
+                 assert (H4: forall x : nat, ~ In x (freeVarF LNN E)).
                  { unfold E; clear H3 E.
                    induction (S (codePrf x0 (notH x) x1)).
                    - simpl; auto.
@@ -790,7 +790,7 @@ End Rosser's_Incompleteness.
 
 Definition RepresentsInSelf (T:System) := 
   exists rep:Formula, exists v:nat,
-    (forall x : nat, In x (freeVarFormula LNN rep) -> x = v)  /\
+    (forall x : nat, In x (freeVarF LNN rep) -> x = v)  /\
       (forall f : Formula,
           mem Formula T f ->
           SysPrf T (substF LNN rep v (natToTerm (codeFormula f)))) /\
